GreedyDeriv/Examples.lean
@@ -17,95 +17,88 @@ instance : Coe String (Loc Char) where
 
 -- a + ab
 def r : Regex (Char) := plus 'a' "ab"
-#eval r.matchEnd "ab"
-#eval r.gmatch "ab"
+#guard r.matchEnd "ab" = r.gmatch "ab"
 
 -- (a + ab)*
 def r2 : Regex (Char) := (plus 'a' "ab").star false
-#eval r2.matchEnd "aab"
-#eval r2.gmatch "aab"
+#guard r2.matchEnd "aab" = r2.gmatch "aab"
 
 -- c + ab
 def r3 : Regex (Char) := plus 'c' (mul 'a' 'b')
-#eval r3.matchEnd "ab"
-#eval r3.gmatch "ab"
+#guard r3.matchEnd "ab" = r3.gmatch "ab"
 
 -- (a + aa)a
 def r4 : Regex (Char) := (plus 'a' "aa").mul 'a'
-#eval r4.matchEnd "aaa"
-#eval r4.gmatch "aaa"
+#guard r4.matchEnd "aaa" = r4.gmatch "aaa"
 
 -- a*a
 def r5 : Regex (Char) := (star 'a' false).mul 'a'
-#eval r5.matchEnd "aa"
-#eval r5.gmatch "aa"
+#guard r5.matchEnd "aa" = r5.gmatch "aa"
 
 -- (ε + b)*
 def r6 : Regex (Char) := (epsilon.plus 'b').star false
-#eval r6.matchEnd "bb"
-#eval r6.gmatch "bb"
+#guard r6.matchEnd "bb" = r6.gmatch "bb"
 
 -- (ε + b)(ε + b)*
 def r6' : Regex (Char) := (epsilon.plus 'b').mul ((epsilon.plus 'b').star false)
-#eval r6'.matchEnd "bb"
-#eval r6'.gmatch "bb"
+#guard r6'.matchEnd "bb" = r6'.gmatch "bb"
 
 -- (a + ε + b)*
 def r7 : Regex (Char) := (plus 'a' (epsilon.plus 'b')).star false
-#eval r7.matchEnd "aaaabbb"
-#eval r7.gmatch "aaaabbb"
+#guard r7.matchEnd "aaaabbb" = r7.gmatch "aaaabbb"
 
 -- (ε + a)b
 def r8 : Regex (Char) := (epsilon.plus 'a').mul 'b'
-#eval r8.matchEnd "ab"
-#eval r8.gmatch "ab"
+#guard r8.matchEnd "ab" = r8.gmatch "ab"
 
 -- ((a + ε + b) + b)
 def r9 : Regex (Char) := Regex.plus ((plus 'a' epsilon).plus 'b') 'b'
-#eval r9.gmatch "b"
-#eval r9.matchEnd "b"
+#guard r9.gmatch "b" = r9.matchEnd "b"
 
 -- (ε + a)*b
 def r10 : Regex (Char) := ((Regex.plus epsilon 'a').star false).mul 'b'
-#eval r10.gmatch "ab"
-#eval r10.matchEnd "ab"
+#guard r10.gmatch "ab" = r10.matchEnd "ab"
 
 -- (a + ε)*(ε + b)
 def r11 : Regex (Char) := ((Regex.plus 'a' epsilon).star false).mul (Regex.plus (epsilon) 'b')
-#eval r11.gmatch "ab"
-#eval r11.matchEnd "ab"
+#guard r11.gmatch "ab" = r11.matchEnd "ab"
 
 -- (ε + a)*(ε + b)
 def r12 : Regex (Char) := ((Regex.plus epsilon 'a').star false).mul (Regex.plus (epsilon) 'b')
-#eval r12.gmatch "ab"
-#eval r12.matchEnd "ab"
+#guard r12.gmatch "ab" = r12.matchEnd "ab"
 
 -- (a + ε + b)*b
 def r13 : Regex (Char) := ((Regex.plus 'a' (Regex.plus epsilon 'b')).star false).mul 'b'
-#eval r13.gmatch "bb"
-#eval r13.matchEnd "bb"
+#guard r13.gmatch "bb" = r13.matchEnd "bb"
 
 -- a*?a
 def r14 : Regex (Char) := (star 'a' true).mul 'a'
-#eval r14.matchEnd "aaa"
-#eval r14.gmatch "aaa"
+#guard r14.matchEnd "aaa" = r14.gmatch "aaa"
 
 -- a*?b
 def r15 : Regex (Char) := (star 'a' true).mul 'b'
-#eval r15.matchEnd "aab"
-#eval r15.gmatch "aab"
+#guard r15.matchEnd "aab" = r15.gmatch "aab"
 
 -- (a + ε + b)*?b
 def r16 : Regex (Char) := (star (plus 'a' (plus epsilon 'b')) true).mul 'b'
-#eval r16.matchEnd "aabb"
-#eval r16.gmatch "aabb"
+#guard r16.matchEnd "aabb" = r16.gmatch "aabb"
 
 -- (aa + aaa)*
 def r17 : Regex (Char) := (star (plus "aa" "aaa") false)
-#eval r17.matchEnd "aaa"
-#eval r17.gmatch "aaa"
+#guard r17.matchEnd "aaa" = r17.gmatch "aaa"
 
 -- (a + b*?)*
 def r18 : Regex Char := (star (plus 'a' (star 'b' true)) false)
-#eval r18.matchEnd "aaabbb"
-#eval r18.gmatch "aaabbb"
+#guard r18.matchEnd "aaabbb" = r18.gmatch "aaabbb"
+
+-- b*(?=b)
+def r19 : Regex Char := (star 'b' false).mul (lookahead 'b')
+#guard r19.matchEnd "bb" = r19.gmatch "bb"
+
+-- (a + ε + b)*(?=b)
+def r20 : Regex (Char) := (star (plus 'a' (plus epsilon 'b')) false).mul (lookahead 'b')
+#guard r20.matchEnd "bb" = r20.gmatch "bb"
+
+-- (?=a)
+def r21 : Regex Char := (lookahead 'a')
+#guard r21.matchEnd "a" = r21.gmatch "a"
